proof/correctness/Properties.ec
@@ -1,0 +1,43 @@
+pragma Goals : printall.
+
+require import AllCore List RealExp IntDiv.
+from Jasmin require import JModel JArray.
+
+require import Types Params Parameters Address Notation Primitives Hash Wots Util.
+require import XMSS_IMPL.
+
+require import Array2 Array3 Array8 Array32 Array64 Array67 Array96 Array2144.
+
+require import Utils. (* valid ptr predicate & addr_to_bytes *)
+require import Correctness_Mem Correctness_Hash. 
+(*---*) import NBytes.
+
+require import Termination Repr.
+
+require import BitEncoding.
+(*---*) import BitChunking.
+
+lemma size_prf : hoare[Hash.prf : true ==> size res = n]
+    by proc; seq 2 : (#pre); auto => />; smt(size_hash).
+
+lemma size_F : hoare[Hash._F : true ==> size res = n]
+    by proc; seq 2: (true); auto => />; smt(size_hash). 
+
+lemma size_chain : hoare[Chain.chain : size X = n ==> size res.`1 = n].
+proof.
+proc.
+sp.
+wp.
+while (size t = n); last by auto => />.  
+seq 3 : (#pre). auto. 
+seq 3 : (#pre /\ size _key = n).
+  + auto => />. call size_prf. skip => />.
+seq 1 : (#pre /\ size bitmask = n). 
+  + auto => />. call size_prf. skip => />.
+auto => />. 
+call size_F.
+skip => />. 
+qed.
+
+lemma ssize_chain : phoare[Chain.chain : size X = n ==> size res.`1 = n] = 1%r 
+    by conseq chain_ll size_chain; auto => />. 
